Coherence.v
@@ -1,10 +1,4 @@
-Require Import Morphisms Base BaseProps Cartesian Equipotence.
-
-Record universe (U : V) : Prop := {
-  universe_empty : empty ∈ U;
-  universe_union : forall x, x ∈ U -> union x ∈ U;
-  universe_powerset : forall x, x ∈ U -> powerset x ∈ U
-}.
+Require Import Morphisms Base BaseProps Cartesian Equipotence Ordinal.
 
 Record small U x : Prop := {
   small_wtn : V;
@@ -13,12 +7,28 @@ Record small U x : Prop := {
   small_inj : injection_def x small_wtn small_fun
 }.
 
-Instance Proper_small : Proper (V_eq ==> V_eq ==> iff) small.
+Lemma small_included_compat : forall U x y, small U x -> y ⊆ x -> small U y.
 Proof.
-apply proper_sym_impl_iff_2; try apply V_eq_sym.
-intros x1 x2 Hx y1 y2 Hy [u f Hu Hf]; exists u f.
-+ rewrite <- Hx; assumption.
-+ rewrite <- Hy; assumption.
+intros U x y [w f Hw Hf] Hm.
+pose (fr := comprehension f (fun p => exists u, exists v, p ≅ tuple u v /\ u ∈ y)).
+assert (Hfr : forall u v, tuple u v ∈ fr <-> (tuple u v ∈ f /\ u ∈ y)).
+{ intros u v; split; intros H.
+  + apply comprehension_spec in H; [|repeat intro; repeat (f_equiv; intro); repeat f_equiv; assumption].
+    destruct H as [? [? [? [Heq ?]]]].
+    split; [assumption|apply tuple_inj_l in Heq; rewrite Heq; intuition].
+  + apply comprehension_spec; [repeat intro; repeat (f_equiv; intro); repeat f_equiv; assumption|].
+    split; [now intuition|].
+    exists u, v; split; intuition.
+}
+exists w fr; [assumption|]; destruct Hf as [Hf1 Hf2 Hf3]; split.
++ intros u Hu.
+  destruct (Hf1 u) as [v [Hv Hp]]; [eapply mem_included_compat; eassumption|].
+  exists v; split; [assumption|].
+  apply Hfr; now intuition.
++ intros u v1 v2 Hv1 Hv2; apply Hfr in Hv1; apply Hfr in Hv2.
+  eapply Hf2; intuition eauto.
++ intros u1 u2 v Hu1 Hu2; apply Hfr in Hu1; apply Hfr in Hu2.
+  eapply Hf3; intuition eauto.
 Qed.
 
 (* Lemma toto : forall x, small omega x ->
@@ -67,8 +77,65 @@ Definition web A := union A.
 Record coherent_def A : Prop := {
   coherent_def_bin : forall x,
     (forall x1 x2, x1 ∈ x -> x2 ∈ x -> cup x1 x2 ∈ A) -> union x ∈ A;
-  coherent_def_stb : forall x1 x2, x1 ∈ A -> x2 ∈ A -> cup x1 x2 ∈ A -> cap x1 x2 ∈ A
+  coherent_def_stb : forall x1 x2, x1 ∈ A -> x2 ⊆ x1 -> x2 ∈ A
 }.
+
+Definition coherent_def_alt (A : V) (R : V -> V -> Prop) : Prop := forall x, x ∈ A -> R x x.
+
+Definition to_alt A := (union A, fun x y => pair x y ∈ A).
+
+Definition of_alt A (R : V -> V -> Prop) :=
+  comprehension (powerset A) (fun a => forall x y, x ∈ a -> y ∈ a -> R x y).
+
+Lemma of_alt_sound : forall A R, Proper (V_eq ==> V_eq ==> iff) R ->
+  coherent_def_alt A R -> coherent_def (of_alt A R).
+Proof.
+assert (HP : forall (R : V -> V -> Prop),
+  Proper (V_eq ==> iff) (fun a => forall x y, x ∈ a -> y ∈ a -> R x y)).
+{ intros R; apply proper_sym_impl_iff; [apply V_eq_sym|].
+  intros x1 x2 Hx H x y; rewrite <- Hx; intuition. }
+intros A R HR Hc; split.
++ intros x Hx; apply comprehension_spec; [now auto|split].
+  - apply powerset_spec; apply included_spec; intros z Hz.
+    apply union_spec in Hz; destruct Hz as [u [Hz Hu]].
+    specialize (Hx _ _ Hu Hu); rewrite cup_idem in Hx.
+    apply comprehension_spec in Hx; [|now auto].
+    eapply mem_included_compat; [eassumption|]; apply powerset_spec; intuition.
+  - intros u1 u2 Hu1 Hu2.
+    apply union_spec in Hu1; destruct Hu1 as [z1 [Hu1 Hz1]].
+    apply union_spec in Hu2; destruct Hu2 as [z2 [Hu2 Hz2]].
+    specialize (Hx z1 z2 Hz1 Hz2); apply comprehension_spec in Hx; [|now auto].
+    apply Hx; apply cup_spec; intuition.
++ intros x1 x2 Hx1 Hm.
+  apply comprehension_spec in Hx1; [|now auto].
+  apply comprehension_spec; [now auto|]; split.
+  - apply powerset_spec; transitivity x1; [eassumption|]; apply powerset_spec; intuition.
+  - intros x y Hx Hy; apply Hx1; eapply mem_included_compat; eassumption.
+Qed.
+
+Lemma to_alt_sound : forall A,
+  coherent_def A -> coherent_def_alt (fst (to_alt A)) (snd (to_alt A)).
+Proof.
+intros A HA; unfold to_alt; simpl; intros x Hx.
+apply union_spec in Hx; destruct Hx as [z [Hx Hz]].
+destruct HA as [HAl HAr]; apply (HAr (union (singleton z))).
++ apply HAl; intros z1 z2 Hz1 Hz2; apply singleton_spec in Hz1; apply singleton_spec in Hz2.
+  rewrite Hz1, Hz2, cup_idem; assumption.
++ apply included_spec; intros u Hu; apply pair_spec in Hu.
+  assert (Hrw : u ≅ x) by intuition; rewrite Hrw in *; clear u Hu Hrw.
+  apply union_spec; exists z; split; [assumption|apply singleton_spec; reflexivity].
+Qed.
+
+Definition coh_le A B :=
+  union A ⊆ union B /\ (forall a, a ⊆ union A -> (a ∈ A <-> a ∈ B)).
+
+Lemma coh_le_included_compat : forall A B, coh_le A B -> A ⊆ B.
+Proof.
+intros A B [Hl Hr]; apply included_spec; intros a Ha.
+apply Hr; [|assumption].
+apply included_spec; intros α Hα; apply union_spec.
+exists a; intuition.
+Qed.
 
 Definition coh_nul := singleton empty.
 
@@ -88,22 +155,186 @@ split.
     destruct Hz as [m [Hz Hm]].
     rewrite (He _ Hm) in Hz; apply empty_spec in Hz; contradiction.
   - intros z Hz; apply empty_spec in Hz; contradiction.
-+ intros x1 x2 Hx1 Hx2 Hx; apply singleton_spec.
-  apply singleton_spec in Hx1; apply singleton_spec in Hx2; rewrite Hx1, Hx2.
++ intros x1 x2 Hx1 Hm; apply singleton_spec.
+  apply singleton_spec in Hx1; rewrite Hx1 in Hm; clear x1 Hx1.
   apply extensionality; apply included_spec; intros z Hz.
-  - apply cap_spec in Hz; destruct Hz as [Hz _]; apply empty_spec in Hz; contradiction.
+  - apply (mem_included_compat _ _ _ Hz) in Hm; assumption.
   - apply empty_spec in Hz; contradiction.
 Qed.
 
-Definition bang U A := comprehension (powerset A)
-  (fun s => (union s ∈ A) /\ (forall a, a ∈ s -> small U a)).
+Definition coh_bang U A := comprehension (powerset A)
+  (fun a => (forall x, x ∈ a -> (small U x)) /\ union a ∈ A).
 
-Lemma coherent_bang : forall U A, coherent_def A -> coherent_def (bang U A).
+Lemma coherent_bang : forall U A, coherent_def A -> coherent_def (coh_bang U A).
 Proof.
+assert (HP : forall U A,
+  Proper (V_eq ==> iff) (fun a => (forall x, x ∈ a -> (small U x)) /\ union a ∈ A)).
+{ intros U A x1 x2 Hx; repeat f_equiv; [|assumption].
+  split; intros H x; [rewrite <- Hx|rewrite Hx]; intuition. }
 intros U A [Hl Hr]; split.
-+ intros x Hx; apply comprehension_spec.
-  { repeat intro; repeat f_equiv; try assumption. admit. }
++ intros a Ha; apply comprehension_spec; [now auto|].
   split; [|split].
-  - apply powerset_spec; apply included_spec; intros z Hz; apply union_spec in Hz.
-    destruct Hz as [u [Hz Hu]].
-  split
+  - apply powerset_spec; apply included_spec; intros z Hz.
+    apply union_spec in Hz; destruct Hz as [u [Hz Hu]].
+    specialize (Ha _ _ Hu Hu); rewrite cup_idem in Ha.
+    apply comprehension_spec in Ha; [|now auto].
+    destruct Ha as [Ha _]; apply powerset_spec in Ha.
+    eapply mem_included_compat; eassumption.
+  - intros u Hu; apply union_spec in Hu; destruct Hu as [x [Hu Hx]].
+    specialize (Ha _ _ Hx Hx); rewrite cup_idem in Ha.
+    apply comprehension_spec in Ha; [|now auto].
+    destruct Ha as [_ [Ha _]]; apply Ha; assumption.
+  - apply Hl; intros x1 x2 Hx1 Hx2.
+    apply union_spec in Hx1; apply union_spec in Hx2.
+    destruct Hx1 as [z1 [Hx1 Hz1]]; destruct Hx2 as [z2 [Hx2 Hz2]].
+    specialize (Ha _ _ Hz1 Hz2).
+    apply comprehension_spec in Ha; [|auto].
+    destruct Ha as [_ [_ Ha]].
+    apply (coherent_def_stb A (Build_coherent_def _ Hl Hr) _ _ Ha).
+    apply included_spec; intros p Hp; apply cup_spec in Hp.
+    apply union_spec.
+    destruct Hp as [Hp|Hp].
+    { exists x1; split; [assumption|]; apply cup_spec; intuition. }
+    { exists x2; split; [assumption|]; apply cup_spec; intuition. }
++ intros x1 x2 Hx1 Hm; apply comprehension_spec; [now auto|].
+  apply comprehension_spec in Hx1; [|now auto].
+  split; [|split].
+  - apply powerset_spec; apply included_spec; intros z Hz.
+    eapply mem_included_compat; [eassumption|].
+    transitivity x1; [assumption|].
+    apply powerset_spec; intuition.
+  - intros z Hz; apply Hx1.
+    eapply mem_included_compat; eassumption.
+  - apply Hl; intros y1 y2 Hy1 Hy2.
+    apply (Hr (union x1)); [now intuition|].
+    apply included_spec; intros z Hz; apply cup_spec in Hz.
+    apply union_spec; destruct Hz as [Hz|Hz]; [exists y1|exists y2]; intuition;
+    eapply mem_included_compat; eassumption.
+Qed.
+
+Lemma coh_bang_spec : forall U A a,
+  a ∈ coh_bang U A <-> (a ⊆ A /\ union a ∈ A /\ (forall x, x ∈ a -> small U x)).
+Proof.
+assert (HP : forall U A,
+  Proper (V_eq ==> iff) (fun a => (forall x, x ∈ a -> (small U x)) /\ union a ∈ A)).
+{ intros U A x1 x2 Hx; repeat f_equiv; [|assumption].
+  split; intros H x; [rewrite <- Hx|rewrite Hx]; intuition. }
+intros U A a; split; intros H.
++ apply comprehension_spec in H; [|now auto]; split; [|split]; try solve [intuition].
+  apply powerset_spec; intuition.
++ apply comprehension_spec; [now auto|]; split; [|split]; try solve [intuition].
+  apply powerset_spec; intuition.
+Qed.
+
+Lemma coh_bang_monotonous : forall U A B, coh_le A B -> coh_le (coh_bang U A) (coh_bang U B).
+Proof.
+intros U A B [Hl Hr]; split.
++ apply included_spec; intros a Ha; apply union_spec in Ha.
+  destruct Ha as [u [Ha Hu]]; apply union_spec; exists u; split; [assumption|].
+  apply coh_bang_spec in Hu; apply coh_bang_spec.
+  split; [|split]; [| |now intuition].
+  - transitivity A; [|apply coh_le_included_compat; constructor]; intuition.
+  - eapply mem_included_compat; [intuition eauto|].
+    apply coh_le_included_compat; constructor; intuition.
++ intros a Ha.
+Admitted.
+
+Lemma coh_bang_monotonous : forall U A B, A ⊆ B -> coh_bang U A ⊆ coh_bang U B.
+Proof.
+assert (HP : forall U A,
+  Proper (V_eq ==> iff) (fun a => (forall x, x ∈ a -> (small U x)) /\ union a ∈ A)).
+{ intros U A x1 x2 Hx; repeat f_equiv; [|assumption].
+  split; intros H x; [rewrite <- Hx|rewrite Hx]; intuition. }
+intros U A B Hs; apply included_spec; intros a Ha.
+apply comprehension_spec in Ha; [|now auto].
+apply comprehension_spec; [now auto|]; split; [|split].
++ apply powerset_spec; transitivity A; [|assumption].
+  apply powerset_spec; intuition.
++ intuition.
++ eapply mem_included_compat; intuition eauto.
+Qed.
+
+Definition injl x := tuple (ordinal_of_nat 0) x.
+Definition injr y := tuple (ordinal_of_nat 1) y.
+Definition sum x y := cup (collection x injl) (collection y injr).
+
+Definition coh_rel A B s1 s2 :=
+  (exists x1 x2, s1 ≅ injl x1 /\ s2 ≅ injl x2 /\ x1 ∈ A /\ x2 ∈ A) \/
+  (exists y1 y2, s1 ≅ injr y1 /\ s2 ≅ injr y2 /\ y1 ∈ B /\ y2 ∈ B).
+
+Definition coh_sum A B := of_alt (sum (union A) (union B)) (coh_rel (union A) (union B)).
+
+Lemma coherent_sum : forall A B, coherent_def A -> coherent_def B -> coherent_def (coh_sum A B).
+Proof.
+assert (HP : forall A B, Proper (V_eq ==> V_eq ==> iff) (coh_rel A B)).
+{ unfold coh_rel, injl, injr.
+  intros A B x1 x2 Hx y1 y2 Hy; repeat f_equiv; intro u; f_equiv; intro v; f_equiv;
+  repeat f_equiv; assumption. }
+intros A B HA HB; apply of_alt_sound; [now auto|].
+intros x Hx; apply cup_spec in Hx; destruct Hx as [Hx|Hx].
++ apply collection_spec in Hx; [|unfold injl; repeat intro; f_equiv; assumption].
+  destruct Hx as [z [Hx Hz]]; left; exists z, z; intuition.
++ apply collection_spec in Hx; [|unfold injr; repeat intro; f_equiv; assumption].
+  destruct Hx as [z [Hx Hz]]; right; exists z, z; intuition.
+Qed.
+
+Lemma coh_sum_monotonous : forall A B C D, A ⊆ B -> C ⊆ D -> coh_sum A C ⊆ coh_sum B D.
+Proof.
+assert (HP : forall A B, Proper (V_eq ==> V_eq ==> iff) (coh_rel A B)).
+{ unfold coh_rel, injl, injr.
+  intros A B x1 x2 Hx y1 y2 Hy; repeat f_equiv; intro u; f_equiv; intro v; f_equiv;
+  repeat f_equiv; assumption. }
+intros A B C D Hl Hr; apply included_spec; intros z Hz.
+apply comprehension_spec; [|].
+Admitted.
+
+Definition small_basetype U X :=
+  (forall x, x ∈ X -> small U x) /\ (forall x a, x ∈ X -> a ∈ x -> small U a).
+Definition basetype_def U A X :=
+  (forall x1 x2, x1 ∈ X -> x2 ∈ X -> cup x1 x2 ∈ A -> x1 ≅ x2) /\ small_basetype U X.
+Definition basetype U A := comprehension (powerset A) (basetype_def U A).
+
+Definition coh_flat A := of_alt A (fun x y => x ≅ y).
+
+Lemma coherent_flat : forall A, coherent_def (coh_flat A).
+Proof.
+assert (HP : Proper (V_eq ==> iff) (fun a : V => forall x y : V, x ∈ a -> y ∈ a -> x ≅ y)).
+{ apply proper_sym_impl_iff; [apply V_eq_sym|]; intros z1 z2 Hz H u v; rewrite <- Hz; auto. }
+intros A; split.
++ intros x Hx; apply comprehension_spec; [assumption|split].
+  - apply powerset_spec, included_spec; intros z Hz.
+    apply union_spec in Hz; destruct Hz as [y [Hz Hy]].
+    specialize (Hx _ _ Hy Hy); rewrite cup_idem in Hx.
+    apply comprehension_spec in Hx; [|assumption].
+    eapply mem_included_compat; [eassumption|].
+    apply powerset_spec; intuition.
+  - intros u v Hu Hv.
+    apply union_spec in Hu; destruct Hu as [a [Hu Ha]].
+    apply union_spec in Hv; destruct Hv as [b [Hv Hb]].
+    specialize (Hx _ _ Ha Hb).
+    apply comprehension_spec in Hx; [|assumption].
+    apply Hx; apply cup_spec; intuition.
++ intros x1 x2 Hx1 Hm.
+  apply comprehension_spec in Hx1; [|assumption].
+  apply comprehension_spec; [assumption|split].
+  - apply powerset_spec; transitivity x1; [assumption|].
+    apply powerset_spec; intuition.
+  - intros x y Hx Hy; apply Hx1;
+    eapply mem_included_compat; eassumption.
+Qed.
+
+Definition coh_type U A := coh_flat (basetype U A).
+
+Lemma coherent_type : forall U A, coherent_def (coh_type U A).
+Proof.
+intros U A; apply coherent_flat.
+Qed.
+
+
+
+Axiom Hierarchy : nat -> V.
+Axiom Top : V.
+Axiom Hierarchy_mem : forall n, Hierarchy n ∈ Hierarchy (S n).
+Axiom Top_mem : forall n, Hierarchy n ∈ Top.
+Axiom Hierarchy_universe : forall n, universe (Hierarchy n).
+
