Ordinal.v
@@ -1,4 +1,4 @@
-Require Import Relations Wellfounded Base BaseProps.
+Require Import Morphisms Relations Wellfounded Base BaseProps.
 
 Definition transitive_set (x : V) := forall z, z ∈ x -> z ⊆ x.
 
@@ -123,6 +123,107 @@ intros x; split; intros H.
   exists (ordinal_of_nat n); [symmetry; assumption|constructor].
 Qed.
 
+Fixpoint Vfix (f : V -> V -> V) (x : V) : V :=
+match x with
+| V_const X Xf => @V_const X (fun e => f (Xf e) (Vfix f (Xf e)))
+end.
+
+Lemma Vfix_spec : forall f x, Vfix f x ≅ collection x (fun y => f y (Vfix f y)).
+Proof.
+intros f x; destruct x; reflexivity.
+Qed.
+
+Instance Proper_Vfix : Proper ((V_eq ==> V_eq ==> V_eq) ==> V_eq ==> V_eq) Vfix.
+Proof.
+assert (HP : forall X1 Xf1 X2 Xf2 (Hx : @V_const X1 Xf1 ≅ @V_const X2 Xf2)
+  f1 f2 (Hf : (V_eq ==> V_eq ==> V_eq)%signature f1 f2)
+  (Heq : forall e1 e2, Xf1 e1 ≅ Xf2 e2 -> Vfix f1 (Xf1 e1) ≅ Vfix f2 (Xf2 e2)),
+  Vfix f1 (V_const Xf1) ⊆ Vfix f2 (V_const Xf2)).
+{
+  intros X1 Xf1 X2 Xf2 Hx f1 f2 Hf Heq xs Hxs.
+  assert (Hrw : exists α, xs = f1 (Xf1 α) (Vfix f1 (Xf1 α))).
+  { clear - Hxs; simpl in Hxs.
+    let T := type of Hxs in
+    let f := match T with V_rel _ (V_const ?f) => f end in
+    set (F := f) in *; change (exists e, xs = F e).
+    clearbody F; clear - Hxs; pattern xs.
+    eapply (V_rel_inv _ F); [intuition eauto|assumption]. }
+  destruct Hrw as [α Hrw]; rewrite Hrw in *; clear xs Hxs Hrw.
+  pose (Hα := Hx); destruct Hα as [Hα _].
+  specialize (Hα (Xf1 α) (V_rel_def _ _)); destruct Hα as [ys [Hyl Hyr]].
+  assert (Hrw : exists β, ys = Xf2 β).
+  { clear - Hyl; simpl in Hyl.
+    pattern ys; eapply (V_rel_inv _ Xf2); intuition eauto. }
+  destruct Hrw as [β Hrw]; rewrite Hrw in *; clear ys Hrw Hyl.
+  specialize (Heq _ _ Hyr).
+  exists (f2 (Xf2 β) (Vfix f2 (Xf2 β))).
+  - symmetry; apply Hf; assumption.
+  - simpl.
+    let f := match goal with [ |- ?t ε V_const ?f ] => f end in
+    change (f β ε V_const f); constructor.
+}
+intros f1 f2 Hf x1; induction x1 as [X1 X1f IH]; intros [X2 X2f] Hx.
+apply extensionality; apply HP; try assumption.
++ intros; apply IH; assumption.
++ symmetry; assumption.
++ symmetry; assumption.
++ intros; symmetry; apply IH; symmetry; assumption.
+Qed.
+
+
+(* Definition collection_dep x (f : forall y, y ∈ x -> V) :=
+match x return (forall y, y ∈ x -> V) -> V with
+| V_const X Xf => fun f => @V_const X (fun y => f (Xf y) (subrelation_mem_rel _ _ (V_rel_def Xf y)))
+end f.
+
+Lemma collection_dep_spec : forall x y f,
+  y ∈ collection_dep x f <-> exists z, exists (H : z ∈ x), y ≅ f z H.
+Proof.
+Admitted.
+
+Lemma transitive_closure : forall x, {y | forall z, z ∈ y <-> clos_trans _ mem z x}.
+Proof.
+intros x; induction (wf_mem x) as [x _ IH].
+pose (R := collection_dep x (fun y Hy => proj1_sig (IH _ Hy))).
+exists (cup R x); intros z; split; intros Hz.
++ apply cup_spec in Hz; destruct Hz as [Hz|Hz].
+  - apply collection_dep_spec in Hz; destruct Hz as [u [Hm Hu]].
+    destruct (IH u Hm) as [v Hv]; simpl in Hu.
+    replace z with v; [|admit]; clear z Hu.
+    admit.
+  - admit.
++ admit.
+Defined.
+
+Extraction transitive_closure.
+
+Fixpoint transitive_closure x :=
+match x with
+| V_const X Xf => 
+end.
+
+Definition Vω := F (fun _ y => collection y powerset) omega.
+
+Lemma Vω_empty : empty ∈ Vω.
+Proof.
+unfold Vω; rewrite F_spec; apply collection_spec; [admit|].
+exists (ordinal_of_nat 0); split; [apply omega_spec; exists 0; reflexivity|].
+apply extensionality; apply included_spec; intros z Hz.
++ apply empty_spec in Hz; contradiction.
++
+  rewrite F_spec in Hz.
+exfalso; apply collection_spec in Hz; [|admit].
+  destruct Hz as [x [Hz _]].
+  apply collection_spec in Hz; [|admit].
+  destruct Hz as [? [Hz _]]; apply empty_spec in Hz; contradiction.
+Qed.
+
+Lemma Vω_powerset : forall x, x ∈ Vω -> powerset x ∈ Vω.
+Proof.
+intros x Hx; unfold Vω in *.
+rewrite F_spec in Hx; apply collection_spec in Hx; [|admit].
+rewrite F_spec; apply collection_spec; [admit|].
+
 Lemma ordinal_rect : forall P,
   (forall x, ordinal x -> (forall y, y ∈ x -> P y) -> P x) -> forall x, ordinal x -> P x.
 Proof.
@@ -131,3 +232,4 @@ induction (wf_mem x) as [x H IHx].
 apply IH; [assumption|].
 intros y Hy; apply IHx; [assumption|eapply ordinal_mem_compat; eassumption].
 Qed.
+*)
